otway-rees/OYRS.Debug.fst
@@ -9,21 +9,30 @@ open LabeledCryptoAPI
 open LabeledRuntimeAPI
 open LabeledPKI
 open AttackerAPI
-open ORYS.Sessions
-open ORYS.Protocol
+open OYRS.Sessions
+open OYRS.Protocol
 
 
 val benign_attacker:
   unit ->
-  LCrypto unit (pki nsl_preds)
+  LCrypto unit (pki oyrs_preds)
   (requires fun _ -> True)
   (ensures fun _ _ _ -> True)
 
 #set-options "--z3rlimit 200 --max_fuel 4 --max_ifuel 2"
 let benign_attacker () =
+  let a:principal = "initiator" in
+  let b:principal = "responder" in
+  let srv:principal = "server" in
+
+  let (|t_as,k_as|) = initiator_init a srv b in
+  let (|t_bs,k_bs|) = responder_init b srv in
+  install_sk_at_auth_server #t_as srv a k_as;
+  install_sk_at_auth_server #t_bs srv b k_bs;
+
   ()
 
-let benign () : LCrypto unit (pki nsl_preds)
+let benign () : LCrypto unit (pki oyrs_preds)
   (requires (fun _ -> True)) (ensures (fun _ _ _ -> True))
 = print_string "start\n";
   let t0 = get() in
@@ -36,7 +45,7 @@ let main =
   IO.print_string "======================\n";
   let t0 = Seq.empty in
   IO.print_string "Starting Benign Attacker:\n";
-  assume(valid_trace (pki nsl_preds) t0);
+  assume(valid_trace (pki oyrs_preds) t0);
   let r,t1 = (reify (benign ()) t0) in
   (match r with
   | Error s -> IO.print_string ("ERROR: "^s^"\n")
