otway-rees/OYRS.Protocol.fsti
@@ -1,15 +1,44 @@
 module OYRS.Protocol
 
 
+open SecrecyLabels
 open CryptoEffect
 open CryptoLib
 open GlobalRuntimeLib
-open ORYS.Messages
-open ORYS.Sessions
+open OYRS.Messages
+open OYRS.Sessions
 open LabeledCryptoAPI
 open LabeledRuntimeAPI
 open LabeledPKI
 
+
+val initiator_init:
+  initiator:principal ->
+  server:principal ->
+  responder:principal ->
+  LCrypto (i:timestamp & secret oyrs_global_usage i (readers [P initiator; P server]) (aead_usage "sk_i_srv")) (pki oyrs_preds)
+  (requires (fun t0 -> True))
+  (ensures (fun t0 (|i,s|) t1 ->
+    i == trace_len t0 /\ trace_len t1 > trace_len t0 /\
+    was_rand_generated_at (trace_len t0) s (readers [P initiator; P server]) (aead_usage "sk_i_srv")))
+
+val responder_init:
+  responder:principal ->
+  server:principal ->
+  LCrypto (i:timestamp & secret oyrs_global_usage i (readers [P responder; P server]) (aead_usage "sk_r_srv")) (pki oyrs_preds)
+  (requires (fun t0 -> True))
+  (ensures (fun t0 (|i,s|) t1 ->
+    i == trace_len t0 /\ trace_len t1 > trace_len t0 /\
+    was_rand_generated_at (trace_len t0) s (readers [P responder; P server]) (aead_usage "sk_r_srv")))
+
+val install_sk_at_auth_server:
+  #i:nat ->
+  server:principal ->
+  p:principal ->
+  sk:(msg oyrs_global_usage i (readers [P p; P server])) ->
+  LCrypto unit (pki oyrs_preds)
+  (requires fun t0 -> i <= trace_len t0)
+  (ensures fun t0 r t1 -> trace_len t1 == trace_len t0 + 1)
 
 val initiator_send_msg_1:
   initiator:principal ->
@@ -21,7 +50,7 @@ val initiator_send_msg_1:
 val responder_send_msg_2:
   responder:principal ->
   message_idx: nat ->
-  LCrypto (state_session_idx:nat * message_idx:nat) (pki orys_preds)
+  LCrypto (state_session_idx:nat * message_idx:nat) (pki oyrs_preds)
   (requires fun t0 ->  message_idx < trace_len t0)
   (ensures fun t0 (si, msg_idx) t1 -> msg_idx < trace_len t1 /\ (trace_len t0 < trace_len t1))
 
@@ -37,7 +66,7 @@ val responder_send_msg_4:
   sess_idx_resp:nat ->
   message_idx:nat ->
   LCrypto (message_idx:nat) (pki oyrs_preds)
-  (requires fun t0 ->  msg_idx < trace_len t0)
+  (requires fun t0 ->  message_idx < trace_len t0)
   (ensures fun t0 msg_idx t1 -> msg_idx < trace_len t1 /\ (trace_len t0 < trace_len t1))
 
 val initiator_recv_msg_4:
